Remove intermediate proofs from the parser
We don't need to pass along a proof that `a <= b` if instead we pass
around `b - a` instead of passing around `a`.  This means the
intermediate steps don't need to talk about proofs, which paves the way
for reflecting the parser term.

After    | File Name                                                | Before   || Change
-------------------------------------------------------------------------------------------
3m55.64s | Total                                                    | 3m39.76s || +0m15.87s
-------------------------------------------------------------------------------------------
0m39.60s | Parsers/GenericRecognizerMin                             | 0m22.67s || +0m16.92s
0m47.43s | Parsers/BooleanRecognizerOptimized                       | 0m49.48s || -0m02.04s
0m09.44s | Parsers/Refinement/SharpenedExpressionPlus               | 0m10.52s || -0m01.08s
0m02.88s | Parsers/GenericRecognizerExt                             | 0m01.39s || +0m01.49s
0m21.45s | Parsers/Refinement/SharpenedJSComment                    | 0m21.54s || -0m00.08s
0m13.32s | Parsers/ParserFromParserADT                              | 0m13.23s || +0m00.08s
0m13.29s | Parsers/Refinement/SharpenedStringLiteral                | 0m12.52s || +0m00.76s
0m12.65s | Parsers/Refinement/SharpenedExpressionPlusParen          | 0m12.22s || +0m00.42s
0m12.61s | Parsers/Refinement/DisjointLemmas                        | 0m12.50s || +0m00.10s
0m07.45s | Parsers/Refinement/SharpenedExpressionParen              | 0m08.24s || -0m00.79s
0m07.42s | Parsers/Refinement/SharpenedExpressionPlusParenParseTree | 0m07.34s || +0m00.08s
0m06.12s | Parsers/Refinement/SharpenedABStar                       | 0m06.19s || -0m00.07s
0m05.52s | Parsers/SimpleRecognizerCorrect                          | 0m05.69s || -0m00.17s
0m03.63s | Parsers/Refinement/BinOpBrackets/BinOpRules              | 0m03.70s || -0m00.07s
0m02.78s | Parsers/ParserImplementation                             | 0m02.76s || +0m00.02s
0m02.54s | Parsers/GenericRecognizerBoolEquality                    | 0m02.54s || +0m00.00s
0m02.39s | Parsers/Refinement/DisjointRules                         | 0m02.29s || +0m00.10s
0m02.20s | Parsers/Refinement/SharpenedABStarParseTree              | 0m02.25s || -0m00.04s
0m02.15s | Parsers/ExtrOcamlParsers                                 | 0m02.12s || +0m00.02s
0m01.96s | Parsers/Refinement/ExtractSharpenedABStar                | 0m01.94s || +0m00.02s
0m01.82s | Parsers/Refinement/Tactics                               | 0m01.68s || +0m00.14s
0m01.73s | Parsers/Refinement/DisjointRulesRev                      | 0m01.60s || +0m00.12s
0m01.63s | Parsers/ParserImplementationOptimized                    | 0m01.65s || -0m00.02s
0m01.56s | Parsers/Refinement/ReductionTactics                      | 0m01.47s || +0m00.09s
0m01.54s | Parsers/GenericRecognizerEquality                        | 0m01.44s || +0m00.10s
0m01.22s | Parsers/BooleanRecognizerEquality                        | 0m01.07s || +0m00.14s
0m01.22s | Parsers/GenericRecognizerCorrect                         | 0m01.17s || +0m00.05s
0m01.20s | Parsers/BooleanRecognizerCorrect                         | 0m01.04s || +0m00.15s
0m01.00s | Parsers/SimpleBooleanRecognizerEquality                  | 0m01.01s || -0m00.01s
0m00.94s | Parsers/SimpleRecognizerExt                              | 0m01.09s || -0m00.15s
0m00.90s | Parsers/BooleanRecognizerExt                             | 0m00.94s || -0m00.03s
0m00.84s | Parsers/BooleanRecognizerTests                           | 0m00.92s || -0m00.08s
0m00.83s | Parsers/GenericRecognizer                                | 0m00.88s || -0m00.05s
0m00.81s | Parsers/SimpleRecognizer                                 | 0m00.92s || -0m00.10s
0m00.80s | Parsers/BooleanRecognizer                                | 0m00.91s || -0m00.10s
0m00.78s | Parsers/BooleanRecognizerFull                            | 0m00.85s || -0m00.06s

src/Parsers/BooleanRecognizer.v
@@ -38,24 +38,19 @@ Section recursive_descent_parser.
          ret_nt_invalid := false }.
 
   Definition parse_item'
-    := Eval cbv [parse_item' parse_nt_T parse_item_T parse_production_T boolean_gendata] in
-        parse_item' str.
+    := parse_item' str.
 
   Definition parse_production'_for {len0}
-    := Eval cbv [parse_production'_for parse_nt_T boolean_gendata parse_production_T] in
-        parse_production'_for str (len0 := len0).
+    := parse_production'_for str (len0 := len0).
 
   Definition parse_production' {len0}
-    := Eval cbv [parse_production' parse_nt_T boolean_gendata parse_production_T] in
-        parse_production' str (len0 := len0).
+    := parse_production' str (len0 := len0).
 
   Definition parse_productions' {len0}
-    := Eval cbv [parse_productions' parse_nt_T boolean_gendata parse_production_T] in
-        parse_productions' str (len0 := len0).
+    := parse_productions' str (len0 := len0).
 
   Definition parse_nonterminal_step {len0 valid_len}
-    := Eval cbv [parse_nonterminal_step parse_nt_T boolean_gendata parse_production_T] in
-        parse_nonterminal_step str (len0 := len0) (valid_len := valid_len).
+    := parse_nonterminal_step str (len0 := len0) (valid_len := valid_len).
 
   Definition parse_nonterminal_or_abort
     : forall (p : nat * nat)
