src/Parsers/BooleanRecognizerExt.v
@@ -14,13 +14,15 @@ Section recursive_descent_parser.
 
   Local Existing Instance boolean_gendata.
 
+  Local Notation nt_ret_T := bool (only parsing).
+
   Global Instance parse_item'_Proper
   : Proper (eq ==> pointwise_relation _ eq ==> eq ==> eq ==> eq ==> eq) (parse_item')
     := parse_item'_Proper.
 
   Definition parse_item'_ext
     : forall (str : String)
-             (str_matches_nonterminal str_matches_nonterminal' : nonterminal_carrierT -> bool)
+             (str_matches_nonterminal str_matches_nonterminal' : nonterminal_carrierT -> _)
              (ext : forall s, str_matches_nonterminal s = str_matches_nonterminal' s)
              (offset : nat)
              (len : nat)
@@ -29,167 +31,77 @@ Section recursive_descent_parser.
       = parse_item' str str_matches_nonterminal' offset len it
     := parse_item'_ext.
 
-  Section production_drop_take.
-    Context {len0}
-            (parse_nonterminal parse_nonterminal'
-             : forall (offset : nat) (len : nat),
-                 len <= len0
-                 -> nonterminal_carrierT
-                 -> bool).
-
-    Definition parse_production'_for_ext_drop_take
-      : forall (str : String)
-               splits splits'
-               (offset : nat)
-               (len : nat)
-               (Hsplits : forall idx len ns, splits idx str (drop_takes_offset ns offset) (drop_takes_len ns len) = splits' idx str (drop_takes_offset ns offset) (drop_takes_len ns len))
-               (ext : forall ns offset len pf nt,
-                   @parse_nonterminal (drop_takes_offset ns offset) (drop_takes_len ns len) pf nt
-                   = @parse_nonterminal' (drop_takes_offset ns offset) (drop_takes_len ns len) pf nt)
-               (ns : list _)
-               (pf pf' : drop_takes_len ns len <= len0)
-               prod_idx,
-        parse_production'_for str parse_nonterminal splits (drop_takes_offset ns offset) pf prod_idx
-        = parse_production'_for str parse_nonterminal' splits' (drop_takes_offset ns offset) pf' prod_idx
-      := parse_production'_for_ext_drop_take parse_nonterminal parse_nonterminal'.
-
-    Definition parse_production'_ext_drop_take
-      : forall (str : String)
-               (offset : nat)
-               (len : nat)
-               (ext : forall ns offset len pf nt,
-                   @parse_nonterminal (drop_takes_offset ns offset) (drop_takes_len ns len) pf nt
-                   = @parse_nonterminal' (drop_takes_offset ns offset) (drop_takes_len ns len) pf nt)
-               (ns : list _)
-               (pf pf' : drop_takes_len ns len <= len0)
-               prod_idx,
-        parse_production' str parse_nonterminal (drop_takes_offset ns offset) pf prod_idx
-        = parse_production' str parse_nonterminal' (drop_takes_offset ns offset) pf prod_idx
-      := parse_production'_ext_drop_take parse_nonterminal parse_nonterminal'.
-  End production_drop_take.
-
   Section production.
-    Context {len0} (str : String)
-            (parse_nonterminal parse_nonterminal'
-             : forall (offset : nat) (len : nat),
-                 len <= len0
-                 -> nonterminal_carrierT
-                 -> bool)
-            (ext : forall offset len pf nt,
-                     parse_nonterminal offset len pf nt
-                     = parse_nonterminal' offset len pf nt).
-
     Definition parse_production'_for_ext
+               {len0} str
+               (parse_nonterminal parse_nonterminal'
+                : forall _ _ _, nt_ret_T)
+               ext
       : forall splits splits'
                (Hsplits : forall idx offset len, splits idx str offset len = splits' idx str offset len)
                (offset : nat)
-               (len : nat)
-               (pf pf' : len <= len0)
+               (len0_minus_len : nat)
                prod_idx,
-        parse_production'_for str parse_nonterminal splits offset pf prod_idx
-        = parse_production'_for str parse_nonterminal' splits' offset pf' prod_idx
+        parse_production'_for (len0 := len0) str parse_nonterminal splits offset len0_minus_len prod_idx
+        = parse_production'_for (len0 := len0) str parse_nonterminal' splits' offset len0_minus_len prod_idx
       := parse_production'_for_ext str _ _ ext.
 
     Definition parse_production'_ext
+               {len0} str
+               (parse_nonterminal parse_nonterminal'
+                : forall _ _ _, nt_ret_T)
+               ext
       : forall (offset : nat)
-               (len : nat)
-               (pf pf' : len <= len0)
+               (len0_minus_len : nat)
                prod_idx,
-        parse_production' str parse_nonterminal offset pf prod_idx
-        = parse_production' str parse_nonterminal' offset pf' prod_idx
+        parse_production' (len0 := len0) str parse_nonterminal offset len0_minus_len prod_idx
+        = parse_production' (len0 := len0) str parse_nonterminal' offset len0_minus_len prod_idx
       := parse_production'_ext str _ _ ext.
   End production.
 
   Global Instance parse_production'_for_Proper {str len0}
-  : Proper ((pointwise_relation _ (forall_relation (fun _ => pointwise_relation _ (pointwise_relation _ eq))))
+  : Proper ((pointwise_relation _ (pointwise_relation _ (pointwise_relation _ eq)))
               ==> (pointwise_relation _ (pointwise_relation _ (pointwise_relation _ (pointwise_relation _ eq))))
               ==> eq
-              ==> forall_relation (fun _ => (fun _ _ => True) ==> eq ==> eq))
+              ==> eq
+              ==> eq
+              ==> eq)
            (parse_production'_for str (len0 := len0))
     := parse_production'_for_Proper.
 
   Global Instance parse_production'_Proper {str len0}
-    : Proper ((pointwise_relation _ (forall_relation (fun _ => pointwise_relation _ (pointwise_relation _ eq))))
+    : Proper ((pointwise_relation _ (pointwise_relation _ (pointwise_relation _ eq)))
                 ==> eq
-                ==> forall_relation (fun _ => (fun _ _ => True) ==> eq ==> eq))
+                ==> eq
+                ==> eq
+                ==> eq)
              (parse_production' str (len0 := len0))
     := parse_production'_Proper.
 
-  Section productions_drop_take.
-    Context {len0} (str : String)
-            (parse_nonterminal parse_nonterminal'
-             : forall (offset : nat)
-                      (len : nat)
-                      (pf : len <= len0),
-                 nonterminal_carrierT -> bool).
-
-    Definition parse_productions'_ext_drop_take
-      : forall (ext : forall ns offset len pf nt,
-                   @parse_nonterminal (drop_takes_offset ns offset) (drop_takes_len ns len) pf nt
-                   = @parse_nonterminal' (drop_takes_offset ns offset) (drop_takes_len ns len) pf nt)
-               (offset : nat)
-               (len : nat)
-               ns
-               (pf pf' : drop_takes_len ns len <= len0)
-               (prods : list production_carrierT),
-        parse_productions' str parse_nonterminal (drop_takes_offset ns offset) pf prods
-        = parse_productions' str parse_nonterminal' (drop_takes_offset ns offset) pf' prods
-      := parse_productions'_ext_drop_take str parse_nonterminal parse_nonterminal'.
-  End productions_drop_take.
-
   Section productions.
-    Context {len0} (str : String)
-            (parse_nonterminal parse_nonterminal'
-             : forall (offset : nat)
-                      (len : nat)
-                      (pf : len <= len0),
-                 nonterminal_carrierT -> bool)
-            (ext : forall str len pf nt,
-                     parse_nonterminal str len pf nt
-                     = parse_nonterminal' str len pf nt).
-
     Definition parse_productions'_ext
+               {len0} str
+               (parse_nonterminal parse_nonterminal'
+                : forall _ _ _, nt_ret_T)
+               ext
       : forall (offset : nat)
-               (len : nat)
-               (pf pf' : len <= len0)
+               (len0_minus_len : nat)
                (prods : list production_carrierT),
-        parse_productions' str parse_nonterminal offset pf prods
-        = parse_productions' str parse_nonterminal' offset pf' prods
+        parse_productions' (len0 := len0) str parse_nonterminal offset len0_minus_len prods
+        = parse_productions' (len0 := len0) str parse_nonterminal' offset len0_minus_len prods
       := parse_productions'_ext str _ _ ext.
   End productions.
 
   Global Instance parse_productions'_Proper {str len0}
-  : Proper ((pointwise_relation _ (forall_relation (fun _ => pointwise_relation _ (pointwise_relation _ eq))))
+  : Proper ((pointwise_relation _ (pointwise_relation _ (pointwise_relation _ eq)))
               ==> eq
-              ==> forall_relation (fun _ => (fun _ _ => True) ==> eq ==> eq))
+              ==> eq
+              ==> eq
+              ==> eq)
            (parse_productions' str (len0 := len0))
     := parse_productions'_Proper.
 
   Section nonterminals.
-    Section step_drop_take.
-      Context {len0 valid_len} (str : String)
-              (parse_nonterminal parse_nonterminal'
-               : forall (p : nat * nat),
-                   Wf.prod_relation lt lt p (len0, valid_len)
-                   -> forall (valid : nonterminals_listT)
-                             (offset : nat) (len : nat),
-                        len <= fst p -> nonterminal_carrierT -> bool).
-
-      Definition parse_nonterminal_step_ext_drop_take
-        : forall (valid : nonterminals_listT)
-                 (ext : forall ns p pf valid offset len pf' nt,
-                     @parse_nonterminal p pf valid (drop_takes_offset ns offset) (drop_takes_len ns len) pf' nt
-                     = @parse_nonterminal' p pf valid (drop_takes_offset ns offset) (drop_takes_len ns len) pf' nt)
-                 (offset : nat)
-                 (len : nat)
-                 ns
-                 (pf pf' : drop_takes_len ns len <= len0)
-                 (nt : nonterminal_carrierT),
-          parse_nonterminal_step str parse_nonterminal valid (drop_takes_offset ns offset) pf nt
-          = parse_nonterminal_step str parse_nonterminal' valid (drop_takes_offset ns offset) pf' nt
-        := parse_nonterminal_step_ext_drop_take str parse_nonterminal parse_nonterminal'.
-    End step_drop_take.
-
     Section step.
       Context {len0 valid_len} (str : String)
               (parse_nonterminal parse_nonterminal'
@@ -197,7 +109,7 @@ Section recursive_descent_parser.
                    Wf.prod_relation lt lt p (len0, valid_len)
                    -> forall (valid : nonterminals_listT)
                              (offset : nat) (len : nat),
-                        len <= fst p -> nonterminal_carrierT -> bool)
+                        len <= fst p -> nonterminal_carrierT -> nt_ret_T)
               (ext : forall p pf valid str len pf' nt,
                        parse_nonterminal p pf valid str len pf' nt
                        = parse_nonterminal' p pf valid str len pf' nt).
