src/Parsers/GenericRecognizerEquality.v
@@ -56,19 +56,19 @@ Section transfer.
   Lemma parse_production_proj
         (len0 : nat)
         parse_nonterminal parse_nonterminal'
-        (H : forall offset len pf' nt,
-               parse_nonterminal offset len pf' nt
-               = parse_nonterminal' offset len pf' nt)
-        offset len pf (prod : @production_carrierT _ data)
-  : @parse_production' _ HSLM_lite _ _ (proj str) len0 parse_nonterminal offset len pf prod
-    = @parse_production' _ HSLM_heavy _ _ str len0 parse_nonterminal' offset len pf prod.
+        (H : forall offset len0_minus_len nt,
+               parse_nonterminal offset len0_minus_len nt
+               = parse_nonterminal' offset len0_minus_len nt)
+        offset len0_minus_len (prod : @production_carrierT _ data)
+  : @parse_production' _ HSLM_lite _ _ (proj str) len0 parse_nonterminal offset len0_minus_len prod
+    = @parse_production' _ HSLM_heavy _ _ str len0 parse_nonterminal' offset len0_minus_len prod.
   Proof.
     unfold parse_production', parse_production'_for.
     simpl.
     set (ls := @to_production Char predata prod).
     generalize (eq_refl : to_production prod = ls).
     clearbody ls.
-    revert prod offset len pf; induction ls; simpl; intros ???? Heq.
+    revert prod offset len0_minus_len; induction ls; simpl; intros ??? Heq.
     { reflexivity. }
     { f_equal; [].
       rewrite split_string_for_production_proj.
@@ -84,12 +84,12 @@ Section transfer.
   Lemma parse_productions_proj
         (len0 : nat)
         parse_nonterminal parse_nonterminal'
-        (H : forall offset len pf' nt,
-               parse_nonterminal offset len pf' nt
-               = parse_nonterminal' offset len pf' nt)
-        offset len pf prods
-  : @parse_productions' _ HSLM_lite _ _ (proj str) len0 parse_nonterminal offset len pf prods
-    = @parse_productions' _ HSLM_heavy _ _ str len0 parse_nonterminal' offset len pf prods.
+        (H : forall offset len0_minus_len nt,
+               parse_nonterminal offset len0_minus_len nt
+               = parse_nonterminal' offset len0_minus_len nt)
+        offset len0_minus_len prods
+  : @parse_productions' _ HSLM_lite _ _ (proj str) len0 parse_nonterminal offset len0_minus_len prods
+    = @parse_productions' _ HSLM_heavy _ _ str len0 parse_nonterminal' offset len0_minus_len prods.
   Proof.
     unfold parse_productions'.
     f_equal; [].
@@ -113,7 +113,7 @@ Section transfer.
     repeat match goal with
              | [ |- appcontext[match ?e with _ => _ end] ]
                => destruct e eqn:?
-             | _ => solve [ erewrite parse_productions_proj; try reflexivity; trivial ]
+             | _ => solve [ erewrite parse_productions_proj; try reflexivity; cbv beta; trivial ]
              | _ => reflexivity
              | _ => progress simpl @option_rect
            end.
